backend/LinearC.v
@@ -55,6 +55,7 @@ End LINEAREXTRA.
 
 Section NEWSTEP.
 
+Variable se: Senv.t.
 Variable ge: genv.
 Let find_function_ptr := find_function_ptr ge.
 
@@ -68,7 +69,7 @@ Definition get_stack (st: state): list stackframe :=
 Inductive step: state -> trace -> state -> Prop :=
 | step_intro
     st0 tr st1
-    (STEP: Linear.step ge st0 tr st1)
+    (STEP: Linear.step se ge st0 tr st1)
     (NOTDUMMY: st1.(get_stack) <> [])
   :
     step st0 tr st1
@@ -408,8 +409,8 @@ End MODSEM.
 Section PROPS.
 
   Lemma step_preserves_last_option
-        ge st0 tr st1 dummy_stack
-        (STEP: step ge st0 tr st1)
+        se ge st0 tr st1 dummy_stack
+        (STEP: step se ge st0 tr st1)
         (LAST: last_option (get_stack st0) = Some dummy_stack)
   :
     <<LAST: last_option (get_stack st1) = Some dummy_stack>>
