cfrontend/UpperBound_B.v
@@ -1,5 +1,5 @@
 Require Import CoqlibC Maps.
-Require Import ASTC Integers Floats Values MemoryC EventsC Globalenvs Smallstep.
+Require Import ASTC Integers Floats Values MemoryC EventsC GlobalenvsC Smallstep.
 Require Import Locations Stacklayout Conventions Linking.
 (** newly added **)
 Require Export Csem Cop Ctypes Ctyping Csyntax Cexec.
@@ -73,7 +73,7 @@ c0 + empty
   Hypothesis WT_EXTERNAL:
     forall id ef args res cc vargs m t vres m',
       In (id, Gfun (External ef args res cc)) prog.(prog_defs) ->
-      external_call ef ge vargs m t vres m' ->
+      external_call ef skenv_link vargs m t vres m' ->
       wt_retval vres res.
 
   Definition local_genv (p : Csyntax.program) :=
@@ -240,6 +240,15 @@ c0 + empty
     induction 1; i; inv ALLOCV2; auto.
     rewrite H in H7. inv H7. eapply IHALLOCV1 in H8. auto.
   Qed.
+
+  Notation "'assign_loc'" := (assign_loc skenv_link) (only parsing).
+  Notation "'bind_parameters'" := (bind_parameters skenv_link) (only parsing).
+  Notation "'rred'" := (rred skenv_link) (only parsing).
+  Notation "'estep'" := (estep skenv_link) (only parsing).
+  (* Let assign_loc := assign_loc skenv_link. *)
+  (* Let bind_parameters := bind_parameters skenv_link. *)
+  (* Let rred := rred skenv_link. *)
+  (* Let estep := estep skenv_link. *)
 
   Lemma assign_loc_determ
         g ty m b
@@ -545,8 +554,6 @@ c0 + empty
     split; intro ASSIGN;
       inv ASSIGN; try (by econs; eauto);
         econs 2; eauto.
-    - rewrite <- volatile_store_same; eauto.
-    - rewrite volatile_store_same; eauto.
   Qed.
 
   Lemma lred_same
@@ -573,11 +580,9 @@ c0 + empty
     - inv RRED; try (by econs); ss
       ; try (by (econs; eauto; rewrite <- deref_loc_same; eauto)).
       + econs; eauto. rewrite <- assign_loc_same; eauto.
-      + econs; eauto. exploit external_call_symbols_preserved; eauto. eapply Senv_equiv2.
     - inv RRED; try (by econs); ss
       ; try (by (econs; eauto; rewrite deref_loc_same; eauto)).
       + econs; eauto. rewrite assign_loc_same; eauto.
-      + econs; eauto. exploit external_call_symbols_preserved; eauto. eapply Senv_equiv1.
   Qed.
 
   Lemma estep_same
@@ -721,6 +726,8 @@ c0 + empty
     Eq. ss.
   Qed.
 
+  Notation "'sstep'" := (sstep skenv_link) (only parsing).
+
   Lemma sstep_same
         st_src tr st0
         (SSTEP: sstep
@@ -743,16 +750,15 @@ c0 + empty
     - (* external call *)
       econs; eauto; ss.
       + exploit function_find_same; eauto.
-      + exploit external_call_symbols_preserved; eauto. eapply Senv_equiv2.
   Qed.
 
   Lemma cstep_same
         st_src tr st0
-        (STEP: Csem.step
+        (STEP: Csem.step skenv_link
                  {| genv_genv := (local_genv prog); genv_cenv := prog_comp_env prog |}
                  st_src tr st0)
     :
-      Csem.step (globalenv prog) st_src tr st0.
+      Csem.step skenv_link (globalenv prog) st_src tr st0.
   Proof.
     inv STEP.
     - econs. exploit estep_same; eauto.
@@ -825,8 +831,32 @@ c0 + empty
       + des_ifs.
         exploit not_external_function_find_same; eauto.
         ss. destruct ef; ss.
-      + exploit external_call_symbols_preserved; eauto. eapply Senv_equiv1.
   Qed.
+
+  Lemma senv_same
+    :
+      ((Genv.globalenv prog): Senv.t) = (skenv_link: Senv.t)
+  .
+  Proof.
+    generalize match_ge_skenv_link; intro MGE.
+    clear - skenv_link LINK_SK_TGT MGE.
+    subst skenv_link. ss. unfold Sk.load_skenv in *. subst tprog. unfold link_sk in *. ss.
+    unfold link_list in *. ss. clarify.
+    inv MGE.
+    apply senv_eta; ss.
+    - uge. apply func_ext1. i. ss.
+    - unfold Genv.public_symbol. uge. apply func_ext1. i. specialize (mge_symb x0). rewrite mge_symb. des_ifs.
+      rewrite mge_pubs. ss.
+    - apply func_ext1. i.
+      destruct (Genv.invert_symbol (Genv.globalenv prog) x0) eqn:T.
+      + apply Genv.invert_find_symbol in T. symmetry. apply Genv.find_invert_symbol. uge. rewrite mge_symb. ss.
+      + destruct (Genv.invert_symbol (Genv.globalenv (CSk.of_program signature_of_function prog)) x0) eqn:U; ss.
+        apply Genv.invert_find_symbol in U. specialize (mge_symb i). uge. rewrite mge_symb in *.
+        apply Genv.find_invert_symbol in U. congruence.
+    - unfold Genv.block_is_volatile, Genv.find_var_info. apply func_ext1. i.
+      specialize (mge_defs x0). uge. inv mge_defs; ss.
+      destruct x; ss. des_ifs.
+  Qed. 
 
   Lemma progress_step
         st_src frs n t st_src'
@@ -837,8 +867,8 @@ c0 + empty
       exists (tr : trace) (st_tgt1 : Smallstep.state (sem tprog)), Step (sem tprog) (State frs) tr st_tgt1.
   Proof.
     inv MTCHST; inv STEP; ss; exists t.
-    - esplits. econs; ss. econs 1. exploit estep_progress; eauto.
-    - esplits. econs; ss. econs 2. exploit sstep_progress; eauto.
+    - esplits. econs; ss.  econs 1. exploit estep_progress; eauto. rewrite <- senv_same. eauto.
+    - esplits. econs; ss. econs 2. exploit sstep_progress; eauto. rewrite <- senv_same. eauto.
     - inv INITSRC; inv INITTGT; inv H.
     - inv INITSRC; inv INITTGT; inv H.
   Qed.
@@ -925,12 +955,12 @@ c0 + empty
   Lemma preservation_prog
         st0 tr st1
         (WT: wt_state ge st0)
-        (STEP: Csem.step ge st0 tr st1)
+        (STEP: Csem.step skenv_link ge st0 tr st1)
     :
       <<WT: wt_state ge st1>>
   .
   Proof.
-    eapply preservation; try refl; eauto.
+    eapply preservation; try apply STEP; try refl; eauto.
     - ii. eapply Genv.find_def_symbol. esplits; eauto.
     - i. admit "ez".
   Qed.
@@ -1061,7 +1091,7 @@ c0 + empty
                ** traceEq.
             ++ right. eapply CIH.
                { econs. ss. }
-               { ss. eapply preservation_prog; eauto. }
+               { ss. eapply preservation_prog; eauto. rewrite <- senv_same. et. }
       + (* initial state *)
         inversion INITSRC; subst; ss.
         left. right. econs; i.
@@ -1192,13 +1222,14 @@ c0 + empty
                         { clear -INIT_MEM m_init ge LINK_SK_TGT tprog H18.
                           induction H18; try (by econs).
                           econs; eauto.
+                          unfold fundef in *. rewrite senv_same in H0.
                           rewrite <- assign_loc_same in H0. eauto. }
                     +++ traceEq.
                 --- (* match state *)
                   right. eapply CIH.
                   { ss. instantiate (1:= 1%nat). inv INITTGT.
                     eapply match_states_intro. ss. }
-                  { ss. eapply preservation_prog; eauto. }
+                  { ss. eapply preservation_prog; eauto. rewrite <- senv_same; et. }
             ++ (* main is syscall *)
               inv SYSMOD. inv INITTGT. ss.
               assert (SAME: sk_tgt = sk_link) by (Eq; auto). clear INITSK.
@@ -1233,15 +1264,15 @@ c0 + empty
                { econs; eauto. }
                { ss. }
           -- (* step_internal *)
-            assert(STEPSRC: Csem.step (globalenv prog) st_src tr st0).
+            assert(STEPSRC: Csem.step skenv_link (globalenv prog) st_src tr st0).
             { exploit cstep_same; eauto. }
             esplits.
-            ++ left. eapply plus_one. eauto.
+            ++ left. eapply plus_one. unfold fundef in *. rewrite senv_same. eauto.
             ++ right. eapply CIH.
                { econs; eauto. }
                { ss. eapply preservation_prog; eauto. }
         * (* progress *)
-          specialize (SAFESRC _ (star_refl _ _ _)). des.
+          specialize (SAFESRC _ (star_refl _ _ _ _)). des.
           -- (* final *)
             inv SAFESRC; inv MTCHST; cycle 1.
             { inv INITTGT. }
@@ -1310,7 +1341,7 @@ c0 + empty
         }
         assert(UB: ~safe (semantics prog) (Csem.Callstate (Vptr b Ptrofs.zero true)
                                                           (Tfunction Tnil type_int32s cc_default) [] Kstop m0)).
-        { ii; ss. specialize (H6 _ (star_refl _ _ _)). des; ss.
+        { ii; ss. specialize (H6 _ (star_refl _ _ _ _)). des; ss.
           - inv H6; ss.
           - rr in NOSTEP. contradict NOSTEP; eauto.
         }
@@ -1373,5 +1404,6 @@ Proof.
     rewrite INTERNAL in *. clarify.
     unfold Genv.find_funct_ptr. des_ifs. }
   { eapply typecheck_program_sound; eauto. }
+  { i. eapply WT_EXTERNAL; et. erewrite <- senv_same in H0; et. ss. et. }
 Qed.
 
